$$
\begin{aligned}
&\mathbf{u}_{t}=-L_{t} \hat{\mathbf{x}}_{t} \\
&L_{t}=\left(B^\top S_{t+1}^{\mathbf{x}} B+R+\sum_{n} C_{n}^\top\left(S_{t+1}^{\mathbf{x}}+S_{t+1}^{\mathrm{e}}\right) C_{n}\right)^{-1} B^\top S_{t+1}^{\mathbf{x}} A \\
&S_{t}^{\mathbf{x}}=Q_{t}+A^\top S_{t+1}^{\mathbf{x}}\left(A-B L_{t}\right) ; \quad S_{T}^{\mathbf{x}}=Q_{T} \\
&S_{t}^{\mathrm{e}}=A^\top S_{t+1}^{\mathbf{x}} B L_t+\left(A-K_{t} H\right)^\top S_{t+1}^{\mathrm{e}}\left(A-K_{t} H\right) ; \quad S_{T}^{\mathrm{e}}=0\\
&s_{t}=\operatorname{tr}\left(S_{t+1}^{\mathrm{x}}\Omega^{\xi}+S_{t+1}^{\mathrm{e}}\left(\Omega^{\xi}+\Omega^{\eta}+K_{t} \Omega^{\omega} K_{t}^{\top}\right)\right)+s_{t+1} ; \quad s_{n}=0 .
\end{aligned}
$$